Uppaal_Networks/AbsInt/Word.thy
@@ -1,0 +1,15 @@
+theory Word
+  imports AbsInt
+begin
+
+section \<open>Abstraction of Machine Words\<close>
+text \<open>More specifically, abstraction for @{type val}, @{type reg} and @{type addr}\<close>
+
+class absword = complete_lattice
+
+locale AbsWord =
+fixes \<gamma>_word :: "('a::absword) \<Rightarrow> int set"
+  assumes mono_gamma: "a \<le> b \<Longrightarrow> \<gamma>_word a \<le> \<gamma>_word b"
+  and gamma_Top[simp]: "\<gamma>_word \<top> = UNIV"
+
+end
