Uppaal_Networks/Notation.thy
@@ -1,0 +1,33 @@
+theory Notation
+  imports HOL.Complete_Lattices
+begin
+
+notation
+  sup (infixl "\<squnion>" 65) and
+  inf (infixl "\<sqinter>" 70) and
+  bot ("\<bottom>") and
+  top ("\<top>") and
+  Inf ("\<Sqinter>") and
+  Sup ("\<Squnion>")
+
+syntax
+  "_INF1"     :: "pttrns \<Rightarrow> 'b \<Rightarrow> 'b"           ("(3INF _./ _)" [0, 10] 10)
+  "_INF"      :: "pttrn \<Rightarrow> 'a set \<Rightarrow> 'b \<Rightarrow> 'b"  ("(3INF _\<in>_./ _)" [0, 0, 10] 10)
+  "_SUP1"     :: "pttrns \<Rightarrow> 'b \<Rightarrow> 'b"           ("(3SUP _./ _)" [0, 10] 10)
+  "_SUP"      :: "pttrn \<Rightarrow> 'a set \<Rightarrow> 'b \<Rightarrow> 'b"  ("(3SUP _\<in>_./ _)" [0, 0, 10] 10)
+
+syntax
+  "_INF1"     :: "pttrns \<Rightarrow> 'b \<Rightarrow> 'b"           ("(3\<Sqinter>_./ _)" [0, 10] 10)
+  "_INF"      :: "pttrn \<Rightarrow> 'a set \<Rightarrow> 'b \<Rightarrow> 'b"  ("(3\<Sqinter>_\<in>_./ _)" [0, 0, 10] 10)
+  "_SUP1"     :: "pttrns \<Rightarrow> 'b \<Rightarrow> 'b"           ("(3\<Squnion>_./ _)" [0, 10] 10)
+  "_SUP"      :: "pttrn \<Rightarrow> 'a set \<Rightarrow> 'b \<Rightarrow> 'b"  ("(3\<Squnion>_\<in>_./ _)" [0, 0, 10] 10)
+
+translations
+  "\<Sqinter>x y. f"   \<rightleftharpoons> "\<Sqinter>x. \<Sqinter>y. f"
+  "\<Sqinter>x. f"     \<rightleftharpoons> "\<Sqinter>(CONST range (\<lambda>x. f))"
+  "\<Sqinter>x\<in>A. f"   \<rightleftharpoons> "CONST Inf ((\<lambda>x. f) ` A)"
+  "\<Squnion>x y. f"   \<rightleftharpoons> "\<Squnion>x. \<Squnion>y. f"
+  "\<Squnion>x. f"     \<rightleftharpoons> "\<Squnion>(CONST range (\<lambda>x. f))"
+  "\<Squnion>x\<in>A. f"   \<rightleftharpoons> "CONST Sup ((\<lambda>x. f) `  A)"
+
+end
