Uppaal_Networks/UPPAAL_Asm_Map.thy
@@ -1,37 +1,6 @@
 theory UPPAAL_Asm_Map
-  imports UPPAAL_Asm
+  imports UPPAAL_Asm Notation
 begin
-
-(* ############# *)
-(* Notation *)
-notation
-  sup (infixl "\<squnion>" 65) and
-  inf (infixl "\<sqinter>" 70) and
-  bot ("\<bottom>") and
-  top ("\<top>") and
-  Inf ("\<Sqinter>") and
-  Sup ("\<Squnion>")
-
-syntax
-  "_INF1"     :: "pttrns \<Rightarrow> 'b \<Rightarrow> 'b"           ("(3INF _./ _)" [0, 10] 10)
-  "_INF"      :: "pttrn \<Rightarrow> 'a set \<Rightarrow> 'b \<Rightarrow> 'b"  ("(3INF _\<in>_./ _)" [0, 0, 10] 10)
-  "_SUP1"     :: "pttrns \<Rightarrow> 'b \<Rightarrow> 'b"           ("(3SUP _./ _)" [0, 10] 10)
-  "_SUP"      :: "pttrn \<Rightarrow> 'a set \<Rightarrow> 'b \<Rightarrow> 'b"  ("(3SUP _\<in>_./ _)" [0, 0, 10] 10)
-
-syntax
-  "_INF1"     :: "pttrns \<Rightarrow> 'b \<Rightarrow> 'b"           ("(3\<Sqinter>_./ _)" [0, 10] 10)
-  "_INF"      :: "pttrn \<Rightarrow> 'a set \<Rightarrow> 'b \<Rightarrow> 'b"  ("(3\<Sqinter>_\<in>_./ _)" [0, 0, 10] 10)
-  "_SUP1"     :: "pttrns \<Rightarrow> 'b \<Rightarrow> 'b"           ("(3\<Squnion>_./ _)" [0, 10] 10)
-  "_SUP"      :: "pttrn \<Rightarrow> 'a set \<Rightarrow> 'b \<Rightarrow> 'b"  ("(3\<Squnion>_\<in>_./ _)" [0, 0, 10] 10)
-
-translations
-  "\<Sqinter>x y. f"   \<rightleftharpoons> "\<Sqinter>x. \<Sqinter>y. f"
-  "\<Sqinter>x. f"     \<rightleftharpoons> "\<Sqinter>(CONST range (\<lambda>x. f))"
-  "\<Sqinter>x\<in>A. f"   \<rightleftharpoons> "CONST Inf ((\<lambda>x. f) ` A)"
-  "\<Squnion>x y. f"   \<rightleftharpoons> "\<Squnion>x. \<Squnion>y. f"
-  "\<Squnion>x. f"     \<rightleftharpoons> "\<Squnion>(CONST range (\<lambda>x. f))"
-  "\<Squnion>x\<in>A. f"   \<rightleftharpoons> "CONST Sup ((\<lambda>x. f) `  A)"
-(* ############*)
 
 subsection "State Map"
 
